src/dafny/utils/Statistics.dfy
@@ -1,0 +1,54 @@
+/*
+ * Copyright 2023 Franck Cassez
+ *
+ * Licensed under the Apache License, Version 2.0 (the "License"); you may
+ * not use this file except in compliance with the License. You may obtain
+ * a copy of the License at http://www.apache.org/licenses/LICENSE-2.0
+ *
+ * Unless required by applicable law or agreed to in writing, software dis-
+ * tributed under the License is distributed on an "AS IS" BASIS, WITHOUT
+ * WARRANTIES OR CONDITIONS OF ANY KIND, either express or implied. See the
+ * License for the specific language governing permissions and limitations
+ * under the License.
+ */
+
+include "./int.dfy"
+
+/**
+  *  Provides statistics for the DFS.
+  */
+module Statistics {
+
+  import Int
+
+  /**   Statistics for the DFS. */
+  datatype Stats = Stats(maxDepthReached: bool := false, visitedStates: nat := 0, wPreInvSuccess: nat := 0, errorState: bool := false) {
+
+    /** Set the indicator that maxDepth is reached to true. */
+    function SetMaxDepth(): Stats {
+      this.(maxDepthReached := true)
+    }
+
+    /** Increment the number of visited states. */
+    function IncVisited(): Stats {
+      this.(visitedStates := this.visitedStates + 1)
+    }
+
+    /** Increment the count of successful WPre checks. */
+    function IncWpre(): Stats {
+      this.(wPreInvSuccess := this.wPreInvSuccess + 1)
+    }
+
+    /** Pretty-print the statistics. */
+    function PrettyPrint(): string {
+      "// MaxDepth reached:" + (if maxDepthReached then "true" else "false") +"\n"
+      + "// ErrorState reached:" + (if errorState then "true" else "false") +"\n"
+      + "// States seen:" + Int.NatToString(visitedStates) + "\n"
+      + "// WPre success:" + Int.NatToString(wPreInvSuccess) + "\n"
+    }
+  }
+
+  /** Default value for Stats. */
+  const DEFAULT_STATS := Stats()
+
+}
